Liquidity record printing fix + BoardroomVoting Extraction (#108)
* liq extraction with chainbase

add liq extraction with chainbase specialization

fix issue with records

* add chainbase specialisation to liq extract

* fix after rebase

* liq extraction with chainbase

add liq extraction with chainbase specialization

fix issue with records

* add chainbase specialisation to liq extract

* fix after rebase

* liq extraction with chainbase

add liq extraction with chainbase specialization

fix issue with records

* BV extraction WIP + add reserved names to pretty-printers

* boardroom extraction WIP

* Boardroom WIP 2

* Boardroom WIP 3

* WIP

* WIP2

* BV extract WIP

* make specialized boardrm for extraction, fix in liq extraction

* Add boardroom extract, fix some bugs in pretty printers

* fix record printing in liquidity + unit tests

execution/examples/BoardroomVotingTest.v
@@ -11,21 +11,41 @@ Require Import LocalBlockchain.
 Require Import Monads.
 Require Import ResultMonad.
 Require Import Serializable.
+Require Import Common. Import AddressMap.
 
 Import ListNotations.
 Import BoardroomMathNotations.
 
+
 Local Open Scope Z.
 Local Open Scope broom.
+
 (*
 Definition modulus : bigZ := 1552518092300708935130918131258481755631334049434514313202351194902966239949102107258669453876591642442910007680288864229150803718918046342632727613031282983744380820890196288509170691316593175367469551763119843371637221007210577919.
 Definition generator : bigZ := 2.
 *)
 Definition modulus : Z := 201697267445741585806196628073.
+Definition four := 4%nat.
+Definition seven := 7%nat.
+Definition _1234583932 := 1234583932.
+Definition _23241 := 23241.
+Definition _159338231 := 159338231.
+
+
+(* Definition modulus : Z := 13. *)
 Definition generator : Z := 3.
 
 Axiom modulus_prime : prime modulus.
-Instance axioms : BoardroomAxioms Z := BigZp.boardroom_axioms modulus modulus_prime.
+Import Lia.
+Module ZAxiomParams <: BoardroomAxiomsZParams.
+  Definition p := modulus.
+  Definition isprime := modulus_prime.
+  Program Definition prime_ge_2 : p >= 2.
+  Proof. easy. Defined.
+End ZAxiomParams.
+Module BVZAxioms := BoardroomAxiomsZ ZAxiomParams. Import BVZAxioms.
+
+Existing Instance boardroom_axioms_Z.
 
 Lemma generator_nonzero : generator !== 0.
 Proof. discriminate. Qed.
@@ -35,20 +55,19 @@ Axiom generator_is_generator :
     ~(z == 0) ->
     exists! (e : Z), (0 <= e < order - 1)%Z /\ pow generator e == z.
 
-Instance generator_instance : Generator axioms :=
+Instance generator_instance : Generator boardroom_axioms_Z :=
   {| BoardroomMath.generator := generator;
      BoardroomMath.generator_nonzero := generator_nonzero;
      generator_generates := generator_is_generator; |}.
 
-Definition num_parties : nat := 7.
-Definition votes_for : nat := 4.
+Definition num_parties : nat := seven.
+Definition votes_for : nat := four.
 
 (* a pseudo-random generator for secret keys *)
-Definition sk n := (Z.of_nat n + 1234583932) * (modulus - 23241)^159338231.
+Definition sk n := (Z.of_nat n + _1234583932) * (modulus - _23241)^_159338231.
 
 (* Make a list of secret keys, here starting at i=7 *)
-Definition sks : list Z :=
-  Eval native_compute in map sk (seq 7 num_parties).
+Definition sks : list Z := map sk (seq seven num_parties).
 
 (* Make a list of votes for each party *)
 Definition svs : list bool :=
@@ -58,21 +77,45 @@ Definition svs : list bool :=
                          (seq 0 (num_parties - votes_for)).
 
 (* Compute the public keys for each party *)
-Definition pks : list Z :=
-  Eval native_compute in map compute_public_key sks.
+Time Definition pks : list Z :=
+  Eval vm_compute in map compute_public_key sks.
 
 Definition rks : list Z :=
-  Eval native_compute in map (reconstructed_key pks) (seq 0 (length pks)).
+  Eval vm_compute in map (reconstructed_key pks) (seq 0 (length pks)).
 
 (* In this example we just use xor for the hash function, which is
    obviously not cryptographically secure. *)
+Definition oneN : N := 1%N.
+
 Definition hash_func (l : list positive) : positive :=
-  N.succ_pos (fold_right (fun p a => N.lxor (Npos p) a) 1%N l).
+  N.succ_pos (fold_left (fun a p => N.lxor (Npos p) a) l oneN).
+
+  
+Definition AddrSize := (2^128)%N.
+Instance Base : ChainBase := LocalChainBase AddrSize.
+Instance ChainBuilder : ChainBuilderType := LocalChainBuilderDepthFirst AddrSize.
+
+Module Params <: BoardroomParams.
+  Definition A : Type := Z.
+  Definition H : list positive -> positive := hash_func.
+  Definition ser : Serializable A := _.
+  Definition axioms : BoardroomAxioms A := _.
+  Definition gen : Generator axioms := _.
+  Axiom d : DiscreteLog axioms gen.
+  Definition discr_log : DiscreteLog axioms gen := d.
+  Definition Base := Base .
+End Params.
+
+Module BV := BoardroomVoting Params. Import BV.
 
 (* Compute the signup messages that would be sent by each party.
    We just use the public key as the chosen randomness here. *)
-Definition signups : list Msg :=
-  Eval native_compute in map (fun '(sk, pk, i) => make_signup_msg hash_func sk 5 i)
+Definition _3 := 3%nat.
+Definition _5 := 5.
+Definition _11 := 11.
+
+Time Definition signups : list Msg :=
+  Eval vm_compute in map (fun '(sk, pk, i) => make_signup_msg sk _5 i)
                              (zip (zip sks pks) (seq 0 (length sks))).
 
 (* Compute the submit_vote messages that would be sent by each party *)
@@ -80,12 +123,8 @@ Definition signups : list Msg :=
    using the make_vote_msg function provided by the contract.
    In this example we just use the secret key as the random parameters. *)
 Definition votes : list Msg :=
-  Eval native_compute in map (fun '(i, sk, sv, rk) => make_vote_msg hash_func pks i sk sv sk sk sk)
+  Eval vm_compute in map (fun '(i, sk, sv, rk) => make_vote_msg pks i sk sv sk sk sk)
                              (zip (zip (zip (seq 0 (length pks)) sks) svs) rks).
-
-Definition AddrSize := (2^128)%N.
-Instance Base : ChainBase := LocalChainBase AddrSize.
-Instance ChainBuilder : ChainBuilderType := LocalChainBuilderDepthFirst AddrSize.
 
 Definition A a :=
   BoundedN.of_Z_const AddrSize a.
@@ -100,16 +139,20 @@ Proof.
               constr:(cons (A z) tail)
     end in
   let num := eval compute in num_parties in
-  let tm := add_addr 11%Z num in
+  let tm := add_addr _11%Z num in
   let tm := eval vm_compute in tm in
   exact tm.
 Defined.
 
+Definition voters_map : AddrMap unit := AddressMap.of_list (map (fun a => (a, tt)) addrs).
+
+Definition five := 5%nat.
+
 Definition deploy_setup :=
-  {| eligible_voters := FMap.of_list (map (fun a => (a, tt)) addrs);
-     finish_registration_by := 3;
+  {| eligible_voters := voters_map;
+     finish_registration_by := _3;
      finish_commit_by := None;
-     finish_vote_by := 5;
+     finish_vote_by := five;
      registration_deposit := 0; |}.
 
 Local Open Scope list.
@@ -125,9 +168,9 @@ Definition boardroom_example : option nat :=
              block_reward := 50; |} in
       option_of_result (builder_add_block chain next_header acts) in
   do chain <- add_block chain [];
-  let dep := build_act creator (create_deployment 0 (boardroom_voting hash_func) deploy_setup) in
+  let dep := build_act creator (create_deployment 0 boardroom_voting deploy_setup) in
   do chain <- add_block chain [dep];
-  do caddr <- hd_error (FMap.keys (lc_contracts (lcb_lc chain)));
+  do caddr <- hd_error (AddressMap.keys (lc_contracts (lcb_lc chain)));
   let send addr m := build_act addr (act_call caddr 0 (serialize m)) in
   let calls := map (fun '(addr, m) => send addr m) (zip addrs signups) in
   do chain <- add_block chain calls;
@@ -135,7 +178,7 @@ Definition boardroom_example : option nat :=
   do chain <- add_block chain votes;
   let tally := build_act creator (act_call caddr 0 (serialize tally_votes)) in
   do chain <- add_block chain [tally];
-  do state <- @contract_state _ (@State _ Z) _ (lcb_lc chain) caddr;
-  BoardroomVoting.tally state.
+  do state <- contract_state (lcb_lc chain) caddr;
+  BV.tally state.
 
 Check (@eq_refl (option nat) (Some votes_for)) <<: boardroom_example = Some votes_for.
